WIP

compose/SimMem.v
@@ -15,7 +15,11 @@ Require Import Integers.
 
 Require Import Skeleton.
 Require Import ModSem.
+Require Import Mod.
 Require Import SimSymb.
+
+Set Implicit Arguments.
+
 
 
 Module SimMem.
@@ -25,7 +29,7 @@ Module SimMem.
     t: Type;
     src_mem: t -> mem;
     tgt_mem: t -> mem;
-    valid: t -> Prop;
+    wf: t -> Prop;
     le: t -> t -> Prop;
     lift: t -> t;
     (* Time order: unlift second arg into first arg. *)
@@ -35,14 +39,14 @@ Module SimMem.
     le_PreOrder :> PreOrder le;
 
     (* lift_le: forall mrel, le mrel (lift mrel); *)
-    lift_valid: forall mrel, valid mrel -> valid (lift mrel);
+    lift_wf: forall mrel, wf mrel -> wf (lift mrel);
     lift_src: forall mrel, (lift mrel).(src_mem) = mrel.(src_mem);
     lift_tgt: forall mrel, (lift mrel).(tgt_mem) = mrel.(tgt_mem);
     unlift_src: forall mrel0 mrel1, (unlift mrel0 mrel1).(src_mem) = mrel1.(src_mem);
     unlift_tgt: forall mrel0 mrel1, (unlift mrel0 mrel1).(tgt_mem) = mrel1.(tgt_mem);
-    unlift_spec: forall mrel0 mrel1, le (lift mrel0) mrel1 -> valid mrel0 -> le mrel0 (unlift mrel0 mrel1);
-    unlift_valid: forall mrel0 mrel1,
-        valid mrel0 -> valid mrel1 -> le (lift mrel0) mrel1 -> valid (unlift mrel0 mrel1);
+    unlift_spec: forall mrel0 mrel1, le (lift mrel0) mrel1 -> wf mrel0 -> le mrel0 (unlift mrel0 mrel1);
+    unlift_wf: forall mrel0 mrel1,
+        wf mrel0 -> wf mrel1 -> le (lift mrel0) mrel1 -> wf (unlift mrel0 mrel1);
 
     sim_val: t -> val -> val -> Prop;
     lift_sim_rel: forall mrel v0 v1, sim_val mrel v0 v1 -> sim_val (lift mrel) v0 v1;
@@ -53,25 +57,39 @@ Module SimMem.
   (* lift_val_rel_list: forall mrel vs0 vs1, val_rel_list mrel vs0 vs1 -> val_rel_list (lift mrel) vs0 vs1; *)
   (* val_rel_int: forall mrel i v, val_rel mrel (Vint i) v -> v = Vint i; *)
 
-    load_exact_preserved: forall
-        ss sk_src sk_tgt
-        (WF: SimSymb.wf ss)
-        (CLOSED: SimSymb.closed ss sk_src sk_tgt)
+    mod_pair_load: forall
+        mp
+        (* (SS: mp.(ModPair.SS) = SS) *)
+        (WF: mp.(ModPair.wf))
         skenv_src skenv_tgt m_src m_tgt
-        (LOADSRC: skenv_src = sk_src.(Sk.load_skenv) /\ sk_src.(Sk.load_mem) = Some m_src)
-        (LOADTGT: skenv_tgt = sk_tgt.(Sk.load_skenv) /\ sk_tgt.(Sk.load_mem) = Some m_tgt)
+        (LOADSRC: skenv_src = mp.(ModPair.src).(Sk.load_skenv) /\ mp.(ModPair.src).(Sk.load_mem) = Some m_src)
+        (LOADTGT: skenv_tgt = mp.(ModPair.tgt).(Sk.load_skenv) /\ mp.(ModPair.tgt).(Sk.load_mem) = Some m_tgt)
       ,
         exists sm,
-          (<<SRCM: sm.(src_mem) = m_src>>) /\
-          (<<TGTM: sm.(tgt_mem) = m_tgt>>) /\
-          (<<EXACT: forall
-              id_src id_tgt b_src b_tgt
-              (SRCFIND: skenv_src.(Genv.find_symbol) id_src = Some b_src)
-              (TGTFIND: skenv_tgt.(Genv.find_symbol) id_tgt = Some b_tgt)
-            ,
-              sm.(sim_val) (Vptr b_src Ptrofs.zero true) (Vptr b_tgt Ptrofs.zero true) <->
-              ss id_src id_tgt>>)
+           (<<SRCM: sm.(src_mem) = m_src>>) /\
+           (<<TGTM: sm.(tgt_mem) = m_tgt>>) /\
+           (<<SIM: mp.(ModPair.ss).(SimSymb.sim_skenv) skenv_src skenv_tgt>>)
     ;
+
+    (* load_exact_preserved: forall *)
+    (*     ss sk_src sk_tgt *)
+    (*     (WF: SimSymb.wf ss) *)
+    (*     skenv_src skenv_tgt m_src m_tgt *)
+    (*     (LOADSRC: skenv_src = sk_src.(Sk.load_skenv) /\ sk_src.(Sk.load_mem) = Some m_src) *)
+    (*     (LOADTGT: skenv_tgt = sk_tgt.(Sk.load_skenv) /\ sk_tgt.(Sk.load_mem) = Some m_tgt) *)
+    (*   , *)
+    (*     exists sm, *)
+    (*       (<<SRCM: sm.(src_mem) = m_src>>) /\ *)
+    (*       (<<TGTM: sm.(tgt_mem) = m_tgt>>) /\ *)
+    (*       (<<SIM: ss.(SimSymb.sim_skenv) skenv_src skenv_tgt>>) *)
+    (*       (* (<<EXACT: forall *) *)
+    (*       (*     id_src id_tgt b_src b_tgt *) *)
+    (*       (*     (SRCFIND: skenv_src.(Genv.find_symbol) id_src = Some b_src) *) *)
+    (*       (*     (TGTFIND: skenv_tgt.(Genv.find_symbol) id_tgt = Some b_tgt) *) *)
+    (*       (*   , *) *)
+    (*       (*     sm.(sim_val) (Vptr b_src Ptrofs.zero true) (Vptr b_tgt Ptrofs.zero true) <-> *) *)
+    (*       (*     ss id_src id_tgt>>) *) *)
+    (* ; *)
   }
   .
 
@@ -85,138 +103,112 @@ Module SimMem.
 
 End SimMem.
 
-Record t' := mkrelation {
-  src_mem: mem;
-  tgt_mem: mem;
-}.
 
-Program Instance MemRelId : SimMem.class ss_ident :=
-{
-  t := t';
-  src_mem := src_mem;
-  tgt_mem := tgt_mem;
-  valid := fun (rel: t') => rel.(src_mem) = rel.(tgt_mem);
-  le := fun (mrel0 mrel1: t') => True;
-  lift := id;
-  unlift := fun _ => id;
-  sim_val := fun (_: t') => eq;
-}.
-Next Obligation.
-  ss.
-Qed.
-Next Obligation.
-  eexists (mkrelation _ _).
-  esplits; ss; eauto.
-  ii.
-  
-Qed.
+(* Program Instance sm_ident: SimMem.class ss_ident := *)
+(* { *)
+(* } *)
 
 
-Program Instance sm_ident: SimMem.class ss_ident :=
-{
-}
+(* Inductive senv_incl (se0 se1: Senv.t): Prop := *)
+(* | senv_incl_intro *)
+(*     (INCL: forall *)
+(*         id b *)
+(*         (FIND: se0.(Senv.find_symbol) id = Some b) *)
+(*       , *)
+(*         <<FIND: se1.(Senv.find_symbol) id = Some b>>) *)
+(* . *)
+
+(* Module PLAYGROUND. *)
+
+(*   Definition blockinj := block -> option block. *)
+
+(*   Inductive compat `{SM: SimMem} (sm0: t) (bi0: blockinj) (ms_src: ModSem.t) (ms_tgt: ModSem.t): Prop := *)
+(*   | compat_intro *)
+(*       (COMPAT: forall *)
+(*           b_src b_tgt *)
+(*           (INSRC: List.In b_tgt ms_src.(ModSem.internals)) *)
+(*           (INTGT: List.In b_src ms_tgt.(ModSem.internals)) *)
+(*         , *)
+(*           sm0.(sim_val) (Vptr b_src Ptrofs.zero true) (Vptr b_tgt Ptrofs.zero true) <-> *)
+(*           bi0 b_src = Some b_tgt) *)
+(*   . *)
+
+(*   (* Lemma compat_le *) *)
+(*   (*       `{SM: SimMem} *) *)
+(*   (*       sm *) *)
+(*   (*       bi bi_linked *) *)
+(*   (*       (SYMB: True (* BI_INCL *)) *) *)
+(*   (*       (******* ############################# SkEnv? GenvLinked? unity with symbinj_linked *) *) *)
+(*   (*       se_src skenv_src *) *)
+(*   (*       (SENVSRC: senv_incl se_src skenv_src) *) *)
+(*   (*       se_tgt skenv_tgt *) *)
+(*   (*       (SENVTGT: senv_incl se_tgt skenv_tgt) *) *)
+(*   (*       (COMPAT: compat sm bi_linked skenv_src skenv_tgt) *) *)
+(*   (*   : *) *)
+(*   (*     <<COMPAT: compat sm bi se_src se_tgt>> *) *)
+(*   (* . *) *)
+(*   (* Proof. *) *)
+(*   (*   inv COMPAT. *) *)
+(*   (*   econs; eauto. *) *)
+(*   (*   i. exploit COMPAT0; eauto. *) *)
+(*   (*   { eapply SENVSRC; eauto. } *) *)
+(*   (*   { eapply SENVTGT; eauto. } *) *)
+(*   (*   i. erewrite H. *) *)
+(*   (*   split; i. *) *)
+(*   (*   - (* linked$ id is some *) *) *)
+(*   (*     rewrite <- H0. *) *)
+(*   (*     (* 1) Senv.find_symbol id is Some -> I linked it. should be same. *) *) *)
+(*   (*     (* 2) Senv.find_symbol id is None -> I didn't link it. *) *) *)
+(*   (*     admit "". *) *)
+(*   (*   - eapply SYMB; eauto. *) *)
+(*   (* Abort. *) *)
 
 
-Inductive senv_incl (se0 se1: Senv.t): Prop :=
-| senv_incl_intro
-    (INCL: forall
-        id b
-        (FIND: se0.(Senv.find_symbol) id = Some b)
-      ,
-        <<FIND: se1.(Senv.find_symbol) id = Some b>>)
-.
-
-Module PLAYGROUND.
-
-  Definition blockinj := block -> option block.
-
-  Inductive compat `{SM: SimMem} (sm0: t) (bi0: blockinj) (ms_src: ModSem.t) (ms_tgt: ModSem.t): Prop :=
-  | compat_intro
-      (COMPAT: forall
-          b_src b_tgt
-          (INSRC: List.In b_tgt ms_src.(ModSem.internals))
-          (INTGT: List.In b_src ms_tgt.(ModSem.internals))
-        ,
-          sm0.(sim_val) (Vptr b_src Ptrofs.zero true) (Vptr b_tgt Ptrofs.zero true) <->
-          bi0 b_src = Some b_tgt)
-  .
-
-  (* Lemma compat_le *)
-  (*       `{SM: SimMem} *)
-  (*       sm *)
-  (*       bi bi_linked *)
-  (*       (SYMB: True (* BI_INCL *)) *)
-  (*       (******* ############################# SkEnv? GenvLinked? unity with symbinj_linked *) *)
-  (*       se_src skenv_src *)
-  (*       (SENVSRC: senv_incl se_src skenv_src) *)
-  (*       se_tgt skenv_tgt *)
-  (*       (SENVTGT: senv_incl se_tgt skenv_tgt) *)
-  (*       (COMPAT: compat sm bi_linked skenv_src skenv_tgt) *)
-  (*   : *)
-  (*     <<COMPAT: compat sm bi se_src se_tgt>> *)
-  (* . *)
-  (* Proof. *)
-  (*   inv COMPAT. *)
-  (*   econs; eauto. *)
-  (*   i. exploit COMPAT0; eauto. *)
-  (*   { eapply SENVSRC; eauto. } *)
-  (*   { eapply SENVTGT; eauto. } *)
-  (*   i. erewrite H. *)
-  (*   split; i. *)
-  (*   - (* linked$ id is some *) *)
-  (*     rewrite <- H0. *)
-  (*     (* 1) Senv.find_symbol id is Some -> I linked it. should be same. *) *)
-  (*     (* 2) Senv.find_symbol id is None -> I didn't link it. *) *)
-  (*     admit "". *)
-  (*   - eapply SYMB; eauto. *)
-  (* Abort. *)
-
-
-End PLAYGROUND.
+(* End PLAYGROUND. *)
 
 
 
-(* Fix: My si. My se_src/se_tgt. *)
-Inductive compat `{SM: SimMem} (sm0: t) (si0: symbinj) (se_src: Senv.t) (se_tgt: Senv.t): Prop :=
-| compat_intro
-    (COMPAT: forall
-        id_src id_tgt b_src b_tgt
-        (SRCB: se_src.(Senv.find_symbol) id_src = Some b_src)
-        (TGTB: se_tgt.(Senv.find_symbol) id_tgt = Some b_tgt)
-      ,
-        sm0.(sim_val) (Vptr b_src Ptrofs.zero true) (Vptr b_tgt Ptrofs.zero true) <->
-        si0$ id_src = Some id_tgt)
-.
+(* (* Fix: My si. My se_src/se_tgt. *) *)
+(* Inductive compat `{SM: SimMem} (sm0: t) (si0: symbinj) (se_src: Senv.t) (se_tgt: Senv.t): Prop := *)
+(* | compat_intro *)
+(*     (COMPAT: forall *)
+(*         id_src id_tgt b_src b_tgt *)
+(*         (SRCB: se_src.(Senv.find_symbol) id_src = Some b_src) *)
+(*         (TGTB: se_tgt.(Senv.find_symbol) id_tgt = Some b_tgt) *)
+(*       , *)
+(*         sm0.(sim_val) (Vptr b_src Ptrofs.zero true) (Vptr b_tgt Ptrofs.zero true) <-> *)
+(*         si0$ id_src = Some id_tgt) *)
+(* . *)
 
-Lemma compat_le
-      `{SM: SimMem}
-      sm
-      si si_linked
-      (SYMB: symbinj_incl si si_linked)
-      (******* ############################# SkEnv? GenvLinked? unity with symbinj_linked *)
-      se_src skenv_src
-      (SENVSRC: senv_incl se_src skenv_src)
-      se_tgt skenv_tgt
-      (SENVTGT: senv_incl se_tgt skenv_tgt)
-      (COMPAT: compat sm si_linked skenv_src skenv_tgt)
-  :
-    <<COMPAT: compat sm si se_src se_tgt>>
-.
-Proof.
-  inv COMPAT.
-  econs; eauto.
-  i. exploit COMPAT0; eauto.
-  { eapply SENVSRC; eauto. }
-  { eapply SENVTGT; eauto. }
-  i. erewrite H.
-  split; i.
-  - (* linked$ id is some *)
-    rewrite <- H0.
-    (* 1) Senv.find_symbol id is Some -> I linked it. should be same. *)
-    (* 2) Senv.find_symbol id is None -> I didn't link it. *)
-    admit "".
-  - eapply SYMB; eauto.
-Abort.
+(* Lemma compat_le *)
+(*       `{SM: SimMem} *)
+(*       sm *)
+(*       si si_linked *)
+(*       (SYMB: symbinj_incl si si_linked) *)
+(*       (******* ############################# SkEnv? GenvLinked? unity with symbinj_linked *) *)
+(*       se_src skenv_src *)
+(*       (SENVSRC: senv_incl se_src skenv_src) *)
+(*       se_tgt skenv_tgt *)
+(*       (SENVTGT: senv_incl se_tgt skenv_tgt) *)
+(*       (COMPAT: compat sm si_linked skenv_src skenv_tgt) *)
+(*   : *)
+(*     <<COMPAT: compat sm si se_src se_tgt>> *)
+(* . *)
+(* Proof. *)
+(*   inv COMPAT. *)
+(*   econs; eauto. *)
+(*   i. exploit COMPAT0; eauto. *)
+(*   { eapply SENVSRC; eauto. } *)
+(*   { eapply SENVTGT; eauto. } *)
+(*   i. erewrite H. *)
+(*   split; i. *)
+(*   - (* linked$ id is some *) *)
+(*     rewrite <- H0. *)
+(*     (* 1) Senv.find_symbol id is Some -> I linked it. should be same. *) *)
+(*     (* 2) Senv.find_symbol id is None -> I didn't link it. *) *)
+(*     admit "". *)
+(*   - eapply SYMB; eauto. *)
+(* Abort. *)
 
 (* Proper migration of below? *)
 (* Hint Rewrite lift_src lift_tgt init_src init_tgt : MR. *)
