compose/SimMemId.v
@@ -1,0 +1,60 @@
+Require Import CoqlibC.
+Require Import Memory.
+Require Import Values.
+Require Import Maps.
+Require Import Events.
+Require Import Globalenvs.
+Require Import sflib.
+Require Import RelationClasses.
+Require Import FSets.
+Require Import Ordered.
+Require Import AST.
+Require Import Asmregs.
+Require Import SymbInj.
+Require Import Integers.
+
+Require Import Skeleton.
+Require Import Mod.
+Require Import ModSem.
+Require Import SimSymb.
+Require Import SimSymbId.
+Require Import SimMem.
+
+Set Implicit Arguments.
+
+
+
+
+Record t' := mkrelation {
+  src_mem: mem;
+  tgt_mem: mem;
+}.
+
+Program Instance MemRelId : SimMem.class SimSymbId :=
+{
+  t := t';
+  src_mem := src_mem;
+  tgt_mem := tgt_mem;
+  valid := fun (rel: t') => rel.(src_mem) = rel.(tgt_mem);
+  le := fun (mrel0 mrel1: t') => True;
+  lift := id;
+  unlift := fun _ => id;
+  sim_val := fun (_: t') => eq;
+}.
+Next Obligation.
+  ss.
+Qed.
+Next Obligation.
+  eexists (mkrelation _ _).
+  esplits; ss; eauto.
+  destruct mp; ss.
+  inv WF. ss.
+  inv WF0. ss. clear_tac.
+  assert(PUBS0: forall id, <<EQ: src.(Mod.sk).(prog_defmap) ! id = tgt.(Mod.sk).(prog_defmap) ! id>>).
+  { i. eapply PUBS. eauto. }
+  clear PUBS.
+  econs; eauto.
+  - admit "This should hold; Maybe ""Genv.init_mem_match"" and ""Genv.init_mem_genv_next"" might help".
+  - admit "This should hold;".
+Qed.
+
